seiostar/Compilation.fst
@@ -11,13 +11,12 @@ open LogRelTargetSource
 module C1 = LogRelTargetSource.CompatibilityLemmas
 module C2 = LogRelSourceTarget.CompatibilityLemmas
 
-let rec compile #g #a (#s:fs_oval g a) (qs:g ⊢ s) : Tot exp (decreases qs) =
+let rec compile #g #a #pre (#s:fs_oval g a pre) (qs:g ⊢ s) : Tot exp (decreases qs) =
   match qs with
   | Qtt -> EUnit
   | QAxiom -> EVar 0
   | QWeaken #g qx -> subst sub_inc (compile qx)
   | QFd fd -> EFileDescr fd
-  | QAppGhost -> EUnit
   | QApp qf qx -> EApp (compile qf) (compile qx)
   | QLambda qbody -> ELam (compile qbody)
   | QFalse -> EFalse
@@ -32,7 +31,9 @@ let rec compile #g #a (#s:fs_oval g a) (qs:g ⊢ s) : Tot exp (decreases qs) =
   | QInr qp -> EInr (compile qp)
   | QCase cond inlc inrc -> ECase (compile cond) (compile inlc) (compile inrc)
   | QLambdaIO qbody -> ELam (compile_ocomp qbody)
-and compile_ocomp #g #a (#s:fs_ocomp g a) (qs:typing_io g s) : Tot exp (decreases qs) =
+  // | QSeqGhost _ _ qk -> compile qk  -- QSeqGhost is commented out in RQ.TypingRelation
+  | QRetype qv -> compile qv
+and compile_ocomp #g #a #pre (#s:fs_ocomp g a pre) (qs:typing_io g s) : Tot exp (decreases qs) =
   match qs with
   | QCall o qargs -> ECall o (compile qargs)
   | QReturn qx -> compile qx
@@ -41,171 +42,181 @@ and compile_ocomp #g #a (#s:fs_ocomp g a) (qs:typing_io g s) : Tot exp (decrease
   | QIfIO qc qt qe -> EIf (compile qc) (compile_ocomp qt) (compile_ocomp qe)
   | QCaseIO qcond qinlc qinrc -> ECase (compile qcond) (compile_ocomp qinlc) (compile_ocomp qinrc)
 
-let rec lem_compile_superset #g (#a:qType) (#s:fs_oval g a) (qs:g ⊢ s)
+let rec lem_compile_superset #g #pre (#a:qType) (#s:fs_oval g a pre) (qs:g ⊢ s)
   : Lemma (ensures (s ⊐ (compile qs))) (decreases qs)
   = match qs with
   | Qtt -> C1.compat_oval_unit g
   | QAxiom #g' #_ -> C1.compat_oval_axiom g' a
-  | QWeaken #g' #_ #b #x qx ->
+  | QWeaken #g' #_ #b #pre' #x qx ->
     lem_compile_superset qx;
-    C1.compat_weaken #g' #a #b x (compile qx)
+    C1.compat_weaken #g' #a #b #pre' x (compile qx)
   | QFd fd -> C1.compat_oval_file_descr g fd
-  | QAppGhost -> C1.compat_oval_unit g
-  | QApp #_ #qa #qb #f #x qf qx ->
+  | QApp #_ #qa #qb #preF #_ #f #preX #x qf qx ->
     lem_compile_superset qf;
     lem_compile_superset qx;
-    C1.compat_oval_app f x (compile qf) (compile qx)
-  | QLambda #_ #_ #_ #body qbody ->
+    C1.compat_oval_app #_ #preF #preX #qa #qb f x (compile qf) (compile qx)
+  | QLambda #_ #_ #_ #_ #body qbody ->
     lem_compile_superset qbody;
     C1.compat_oval_lambda body (compile qbody)
   | QFalse -> C1.compat_oval_false g
   | QTrue -> C1.compat_oval_true g
   | QStringLit #_ str -> C1.compat_oval_string g str
-  | QStringEq #_ #s1 qs1 #s2 qs2 ->
+  | QStringEq #_ #_ #s1 qs1 #_ #s2 qs2 ->
     lem_compile_superset qs1;
     lem_compile_superset qs2;
     C1.compat_oval_string_eq s1 s2 (compile qs1) (compile qs2)
-  | QIf #_ #_ #c qc #t qt #e qe ->
+  | QIf #_ #_ #_ #c qc #_ #t qt #_ #e qe ->
     lem_compile_superset qc;
     lem_compile_superset qt;
     lem_compile_superset qe;
     C1.compat_oval_if c t e (compile qc) (compile qt) (compile qe)
-  | QMkpair #_ #a1 #a2 #s1 #s2 q1 q2 ->
+  | QMkpair #_ #a1 #a2 #_ #s1 #_ #s2 q1 q2 ->
     lem_compile_superset q1;
     lem_compile_superset q2;
     C1.compat_oval_pair s1 s2 (compile q1) (compile q2)
-  | QFst #_ #_ #_ #p qp ->
+  | QFst #_ #_ #_ #_ #p qp ->
     lem_compile_superset qp;
     C1.compat_oval_pair_fst p (compile qp)
-  | QSnd #_ #_ #_ #p qp ->
+  | QSnd #_ #_ #_ #_ #p qp ->
     lem_compile_superset qp;
     C1.compat_oval_pair_snd p (compile qp)
-  | QInl #_ #_ #t2 #p qp ->
+  | QInl #_ #_ #t2 #_ #p qp ->
     lem_compile_superset qp;
     C1.compat_oval_inl t2 p (compile qp)
-  | QInr #_ #t1 #_ #p qp ->
+  | QInr #_ #t1 #_ #_ #p qp ->
     lem_compile_superset qp;
     C1.compat_oval_inr t1 p (compile qp)
-  | QCase #_ #_ #_ #_ #cond qcond #inlc qinlc #inrc qinrc ->
+  | QCase #_ #_ #_ #_ #_ #cond qcond #_ #inlc qinlc #_ #inrc qinrc ->
     lem_compile_superset qcond;
     lem_compile_superset qinlc;
     lem_compile_superset qinrc;
     C1.compat_oval_case cond inlc inrc (compile qcond) (compile qinlc) (compile qinrc)
-  | QLambdaIO #_ #_ #_ #body qbody ->
+  | QLambdaIO #_ #_ #_ #_ #body qbody ->
     lem_compile_superset_comp qbody;
     C1.compat_oval_lambda_ocomp body (compile_ocomp qbody)
-and lem_compile_superset_comp #g (#a:qType) (#s:fs_ocomp g a) (qs:typing_io g s)
+  // | QSeqGhost _ _ #_ #_ #k qk ->
+  //   lem_compile_superset qk;
+  //   admit ()
+  | QRetype #_ #_ #_ #v qv #b ->
+    lem_compile_superset qv;
+    C1.compat_oval_retype v b (compile qv)
+and lem_compile_superset_comp #g #pre (#a:qType) (#s:fs_ocomp g a pre) (qs:typing_io g s)
   : Lemma (ensures (s ⊒ (compile_ocomp qs))) (decreases qs)
   =
   match qs with
-  | QCall o #args qargs ->
+  | QCall o #_ #args qargs ->
     lem_compile_superset qargs;
     C1.compat_ocomp_call_oval o args (compile qargs)
-  | QReturn #_ #_ #x qx ->
+  | QReturn #_ #_ #_ #x qx ->
     lem_compile_superset qx;
     C1.compat_ocomp_return x (compile qx)
-  | QBind #_ #_ #_ #m #k qm qk ->
+  | QBind #_ #_ #_ #_ #m #_ #k qm qk ->
     lem_compile_superset_comp qm;
     lem_compile_superset_comp qk;
     C1.compat_ocomp_bind m k (compile_ocomp qm) (compile_ocomp qk)
-  | QAppIO #_ #_ #_ #f #x qf qx ->
+  | QAppIO #_ #_ #_ #_ #f #_ #x qf qx ->
     lem_compile_superset qf;
     lem_compile_superset qx;
     C1.compat_ocomp_app_oval_oval f x (compile qf) (compile qx)
-  | QIfIO #_ #_ #c qc #t qt #e qe ->
+  | QIfIO #_ #_ #_ #c qc #_ #t qt #_ #e qe ->
     lem_compile_superset qc;
     lem_compile_superset_comp qt;
     lem_compile_superset_comp qe;
     C1.compat_ocomp_if_oval c t e (compile qc) (compile_ocomp qt) (compile_ocomp qe)
-  | QCaseIO #_ #_ #_ #_ #cond qcond #inlc qinlc #inrc qinrc ->
+  | QCaseIO #_ #_ #_ #_ #_ #cond qcond #_ #inlc qinlc #_ #inrc qinrc ->
     lem_compile_superset qcond;
     lem_compile_superset_comp qinlc;
     lem_compile_superset_comp qinrc;
     C1.compat_ocomp_case_oval cond inlc inrc (compile qcond) (compile_ocomp qinlc) (compile_ocomp qinrc)
 
-let rec lem_compile_subset #g (#a:qType) (#s:fs_oval g a) (qs:g ⊢ s)
+let rec lem_compile_subset #g #pre (#a:qType) (#s:fs_oval g a pre) (qs:g ⊢ s)
   : Lemma (ensures (s ⊏ (compile qs))) (decreases qs)
   = match qs with
   | Qtt -> C2.compat_oval_unit g
   | QAxiom #g' #_ -> C2.compat_oval_axiom g' a
-  | QWeaken #g' #_ #b #x qx ->
+  | QWeaken #g' #_ #b #preX #x qx ->
     lem_compile_subset qx;
-    C2.compat_weaken #g' #a #b x (compile qx)
+    C2.compat_weaken #g' #a #b #preX x (compile qx)
   | QFd fd -> C2.compat_oval_file_descr g fd
-  | QAppGhost -> C2.compat_oval_unit g
-  | QApp #_ #qa #qb #f #x qf qx ->
+  | QApp #_ #qa #qb #preF #_ #f #preX #x qf qx ->
     lem_compile_subset qf;
     lem_compile_subset qx;
-    C2.compat_oval_app f x (compile qf) (compile qx)
-  | QLambda #_ #_ #_ #body qbody ->
+    C2.compat_oval_app #_ #preF #preX #qa #qb f x (compile qf) (compile qx)
+  | QLambda #_ #_ #_ #_ #body qbody ->
     lem_compile_subset qbody;
     C2.compat_oval_lambda body (compile qbody)
   | QFalse -> C2.compat_oval_false g
   | QTrue -> C2.compat_oval_true g
   | QStringLit #_ str -> C2.compat_oval_string g str
-  | QStringEq #_ #s1 qs1 #s2 qs2 ->
+  | QStringEq #_ #_ #s1 qs1 #_ #s2 qs2 ->
     lem_compile_subset qs1;
     lem_compile_subset qs2;
     C2.compat_oval_string_eq s1 s2 (compile qs1) (compile qs2)
-  | QIf #_ #_ #c qc #t qt #e qe ->
+  | QIf #_ #_ #_ #c qc #_ #t qt #_ #e qe ->
     lem_compile_subset qc;
     lem_compile_subset qt;
     lem_compile_subset qe;
     C2.compat_oval_if c t e (compile qc) (compile qt) (compile qe)
-  | QMkpair #_ #a1 #a2 #s1 #s2 q1 q2 ->
+  | QMkpair #_ #a1 #a2 #_ #s1 #_ #s2 q1 q2 ->
     lem_compile_subset q1;
     lem_compile_subset q2;
     C2.compat_oval_pair s1 s2 (compile q1) (compile q2)
-  | QFst #_ #_ #_ #p qp ->
+  | QFst #_ #_ #_ #_ #p qp ->
     lem_compile_subset qp;
     C2.compat_oval_pair_fst p (compile qp)
-  | QSnd #_ #_ #_ #p qp ->
+  | QSnd #_ #_ #_ #_ #p qp ->
     lem_compile_subset qp;
     C2.compat_oval_pair_snd p (compile qp)
-  | QInl #_ #_ #t2 #p qp ->
+  | QInl #_ #_ #t2 #_ #p qp ->
     lem_compile_subset qp;
     C2.compat_oval_inl t2 p (compile qp)
-  | QInr #_ #t1 #_ #p qp ->
+  | QInr #_ #t1 #_ #_ #p qp ->
     lem_compile_subset qp;
     C2.compat_oval_inr t1 p (compile qp)
-  | QCase #_ #_ #_ #_ #cond qcond #inlc qinlc #inrc qinrc ->
+  | QCase #_ #_ #_ #_ #_ #cond qcond #_ #inlc qinlc #_ #inrc qinrc ->
     lem_compile_subset qcond;
     lem_compile_subset qinlc;
     lem_compile_subset qinrc;
     C2.compat_oval_case cond inlc inrc (compile qcond) (compile qinlc) (compile qinrc)
-  | QLambdaIO #_ #_ #_ #body qbody ->
+  | QLambdaIO #_ #_ #_ #_ #body qbody ->
     lem_compile_subset_comp qbody;
     C2.compat_oval_lambda_ocomp body (compile_ocomp qbody)
-and lem_compile_subset_comp #g (#a:qType) (#s:fs_ocomp g a) (qs:typing_io g s)
+//  | QSeqGhost _ _ #_ #_ #k qk ->
+//    lem_compile_subset qk;
+//    admit ()
+  | QRetype #_ #_ #_ #v qv #b ->
+    lem_compile_subset qv;
+    C2.compat_oval_retype v b (compile qv)
+and lem_compile_subset_comp #g #pre (#a:qType) (#s:fs_ocomp g a pre) (qs:typing_io g s)
   : Lemma (ensures (s ⊑ (compile_ocomp qs))) (decreases qs)
   =
   match qs with
-  | QCall o #args qargs ->
+  | QCall o #_ #args qargs ->
     lem_compile_subset qargs;
     C2.compat_ocomp_call_oval o args (compile qargs)
-  | QReturn #_ #_ #x qx ->
+  | QReturn #_ #_ #_ #x qx ->
     lem_compile_subset qx;
     C2.compat_ocomp_return x (compile qx)
-  | QBind #_ #_ #_ #m #k qm qk ->
+  | QBind #_ #_ #_ #_ #m #_ #k qm qk ->
     lem_compile_subset_comp qm;
     lem_compile_subset_comp qk;
     C2.compat_ocomp_bind m k (compile_ocomp qm) (compile_ocomp qk)
-  | QAppIO #_ #_ #_ #f #x qf qx ->
+  | QAppIO #_ #_ #_ #_ #f #_ #x qf qx ->
     lem_compile_subset qf;
     lem_compile_subset qx;
     C2.compat_ocomp_app_oval_oval f x (compile qf) (compile qx)
-  | QIfIO #_ #_ #c qc #t qt #e qe ->
+  | QIfIO #_ #_ #_ #c qc #_ #t qt #_ #e qe ->
     lem_compile_subset qc;
     lem_compile_subset_comp qt;
     lem_compile_subset_comp qe;
     C2.compat_ocomp_if_oval c t e (compile qc) (compile_ocomp qt) (compile_ocomp qe)
-  | QCaseIO #_ #_ #_ #_ #cond qcond #inlc qinlc #inrc qinrc ->
+  | QCaseIO #_ #_ #_ #_ #_ #cond qcond #_ #inlc qinlc #_ #inrc qinrc ->
     lem_compile_subset qcond;
     lem_compile_subset_comp qinlc;
     lem_compile_subset_comp qinrc;
     C2.compat_ocomp_case_oval cond inlc inrc (compile qcond) (compile_ocomp qinlc) (compile_ocomp qinrc)
 
-let rec lem_compile_fv_in_env #g (#a:qType) (#s:fs_oval g a) (qs:g ⊢ s)
+let rec lem_compile_fv_in_env #g #pre (#a:qType) (#s:fs_oval g a pre) (qs:g ⊢ s)
   : Lemma (ensures fv_in_env g (compile qs)) (decreases qs)
   = match qs with
   | Qtt -> ()
@@ -214,7 +225,6 @@ let rec lem_compile_fv_in_env #g (#a:qType) (#s:fs_oval g a) (qs:g ⊢ s)
     lem_compile_fv_in_env qx;
     lem_fv_in_env_weaken g' b (compile qx)
   | QFd _ -> ()
-  | QAppGhost -> ()
   | QApp qf qx ->
     lem_compile_fv_in_env qf;
     lem_compile_fv_in_env qx;
@@ -258,7 +268,11 @@ let rec lem_compile_fv_in_env #g (#a:qType) (#s:fs_oval g a) (qs:g ⊢ s)
   | QLambdaIO #_ #qa #_ #body qbody ->
     lem_compile_fv_in_env_prod qbody;
     lem_fv_in_env_lam g qa (compile_ocomp qbody)
-and lem_compile_fv_in_env_prod #g (#a:qType) (#s:fs_ocomp g a) (qs:typing_io g s)
+//  | QSeqGhost _ _ #_ #_ #k qk ->
+//    lem_compile_fv_in_env qk
+  | QRetype qv ->
+    lem_compile_fv_in_env qv
+and lem_compile_fv_in_env_prod #g #pre (#a:qType) (#s:fs_ocomp g a pre) (qs:typing_io g s)
   : Lemma (ensures fv_in_env g (compile_ocomp qs)) (decreases qs)
   = match qs with
   | QCall o qargs ->
@@ -287,33 +301,33 @@ and lem_compile_fv_in_env_prod #g (#a:qType) (#s:fs_ocomp g a) (qs:typing_io g s
     lem_fv_in_env_case g ta tb (compile qcond) (compile_ocomp qinlc) (compile_ocomp qinrc)
 
 let lem_compile_closed_arrow_is_elam (#a #b:qType) (#s:fs_val (a ^->!@ b))
-  (qs:(a ^->!@ b) ⊩ s)
-  : Lemma (requires (QLambdaIO? qs))
-          (ensures (ELam? (compile qs)))
+  (qs:(a ^->!@ b) ⊫ s)
+  : Lemma (requires (QLambdaIO? qs._3))
+          (ensures (ELam? (compile qs._3)))
   =
-  match qs with
+  match qs._3 with
   | QLambdaIO qbody ->
-    assert (ELam? (compile qs)) by (norm [delta_once [`%compile];zeta;iota])
+    assert (ELam? (compile qs._3)) by (norm [delta_once [`%compile];zeta;iota])
 
-let lem_compile_is_closed (#a:qType) (#s:fs_val a) (qs:a ⊩ s)
-  : Lemma (is_closed (compile qs))
-  = lem_compile_fv_in_env qs
+let lem_compile_is_closed (#a:qType) (#s:fs_val a) (qs:a ⊫ s)
+  : Lemma (is_closed (compile qs._3))
+  = lem_compile_fv_in_env qs._3
 
-let lem_compile_closed_valid (#a:qType) (#s:fs_val a) (qs:a ⊩ s)
+let lem_compile_closed_valid (#a:qType) (#s:fs_val a) (qs:a ⊫ s)
   : Lemma
-    (requires (QLambdaIO? qs))
+    (requires (QLambdaIO? qs._3))
     (ensures (
-        is_closed (compile qs) /\
-        is_value (compile qs) /\
-        valid_contains s (compile qs) /\
-        valid_member_of s (compile qs)
+        is_closed (compile qs._3) /\
+        is_value (compile qs._3) /\
+        valid_contains s (compile qs._3) /\
+        valid_member_of s (compile qs._3)
       )) =
-  match qs with
+  match qs._3 with
   | QLambdaIO #_ #b #c qbody ->
     lem_compile_is_closed qs;
     lem_compile_closed_arrow_is_elam #b #c #s qs;
-    assert (is_value (compile qs));
-    lem_compile_superset qs;
-    lem_value_superset_valid_contains a (fun _ -> s) (compile qs);
-    lem_compile_subset qs;
-    lem_value_subset_valid_member_of a (fun _ -> s) (compile qs)
+    assert (is_value (compile qs._3));
+    lem_compile_superset qs._3;
+    lem_value_superset_valid_contains a #qs._1 (fun _ -> s) (compile qs._3);
+    lem_compile_subset qs._3;
+    lem_value_subset_valid_member_of a (fun _ -> s) (compile qs._3)
